Broken

src/mitchell/group_theory/quot_group.lean
@@ -5,6 +5,14 @@ import mitchell.group_theory.coset mitchell.group_theory.subgroup
 universes u v w
 variables {α : Type u} {β : Type v} {γ : Type w}
 
+namespace classical
+
+lemma some_spec2 {α : Type u} {p : α → Prop} {h : ∃a, p a} (q : α → Prop) (hpq : ∀a, p a → q a) :
+  q (some h) :=
+hpq _ $ some_spec _
+
+end classical
+
 open set
 
 namespace quotient_group
@@ -104,25 +112,67 @@ structure group_isomorphism (β : Type v) (γ : Type w) [group β] [group γ]
 
 infix ` ≃ₕ `:50 := group_isomorphism
 
-def ker_quot_lift [G : group α] [H : group β] {f : α → β} (hf : is_hom f) (q : α / hf.kernel) : β :=
-quot.lift_on q f (begin
-intros a b hs,
-simp [setoid.r, norm_equiv] at hs,
-simp [hf.hom_mul, hf.inv] at hs,
-rw ←inv_inv (f b),
-apply eq_inv_of_mul_eq_one hs
-end)
+def qgroup_lift [G : group α] [H : group β] (N : set α) [hs : is_normal_subgroup N] {f : α → β} (hf : is_hom f) (h : ∀ x ∈ N, f x = 1) (q : α / N) : β :=
+quot.lift_on q f $ assume a b (hab : a * b⁻¹ ∈ N),
+  have f a * (f b)⁻¹ = 1, by rw [←hf.inv, ←hf.hom_mul]; exact h _ hab,
+  show f a = f b, by rw [←inv_inv (f b)]; exact eq_inv_of_mul_eq_one this
 
 @[simp] lemma mul_val [group α] [group β] ( f : α → β ) (a b : image f) [hf : is_hom f] : (a * b).val = a.val * b.val := by sorry
+@[simp] lemma one_val [group α] [group β] ( f : α → β ) [hf : is_hom f] : (1 : image f).val = 1 := sorry
+@[simp] lemma inv_val [group α] [group β] ( f : α → β ) (a : image f) [hf : is_hom f] : (a⁻¹).val = a.val⁻¹ := sorry
 
 def im_lift [G : group α] [H : group β] {f : α → β} (hf : is_hom f) (c : α) : image f := ⟨f c, image_mem f c⟩
 
 lemma is_hom_image [G : group α] [H : group β] {f : α → β} (hf : is_hom f) : is_hom (λ c, im_lift hf c : α → image f) :=
-    by refine {..};  intros; apply subtype.eq; simp [hf.hom_mul]
+    by refine {..};  intros; apply subtype.eq; simp [im_lift, hf.hom_mul]
+
+set_option pp.implicit true
+
+lemma kernel_cosets {α β} [G : group α] [H : group β] (f : α → β ) [h : is_hom f] {a b} (hab : f a = f b) 
+    : @quotient.mk _ (quotient_group_setoid h.kernel) a = @quotient.mk _ (quotient_group_setoid h.kernel) b :=
+begin
+apply quot.sound,
+unfold setoid.r,
+unfold norm_equiv,
+simp,
+sorry -- easy
+end
+
+variable {r : α → α → Prop}
+variable {S : quot r → Sort v}
+
+lemma quot.rec_eq
+   (f : Π a, S (quot.mk r a)) (h : ∀ (a b : α) (p : r a b), (eq.rec (f a) (quot.sound p) : S (quot.mk r b)) = f b)
+   (a : α) : @quot.rec α r S f h (quot.mk r a) = f a := by refl
 
 noncomputable theorem first_isomorphism_theorem [G : group α] [H : group β] (f : α → β ) [h : is_hom f]
     : α / h.kernel ≃ₕ image f := {
-        to_fun := ker_quot_lift (is_hom_image h)
+        to_fun := qgroup_lift h.kernel (is_hom_image h) (assume x hx, subtype.eq $ by simp [im_lift]; exact is_hom.mem_ker_one _ hx),
+        inv_fun := λ b, @quotient.mk _ (quotient_group_setoid _) (classical.some b.2),
+        left_inv := assume b', @quotient.induction_on _ (quotient_group_setoid _) _ b' $
+            begin
+                assume b,
+                apply quotient.sound,
+                simp [im_lift, qgroup_lift],
+                have hz := @classical.some_spec _ (λ z, f z = f b) ⟨b, rfl⟩,
+                unfold has_equiv.equiv,
+                unfold setoid.r,
+                unfold norm_equiv,
+                simp,
+                apply is_hom.inv_ker_one h hz,
+            end,
+        right_inv := assume c, subtype.eq $ begin
+        simp [qgroup_lift, im_lift, quot.lift_on],
+        let a := classical.some c.property,
+        have hc : c = ⟨f a, _⟩, by simp [classical.some_spec c.property],
+        rw hc,
+        simp,
+        have p : @quotient.mk  _ (quotient_group_setoid _) (@classical.some α (λ (x : α), f a = f a) _) = @quotient.mk  _ (quotient_group_setoid _) (a), {
+                          sorry, -- not too hard
+                        },
+        rw quot.rec_eq
+        
+        end
     }
 
 end
